lib/Lib.Bitmap.fst
@@ -2,49 +2,67 @@ module Lib.Bitmap
 
 open Lib.IntTypes
 open Lib.Sliceable
+open Lib.Circuits
+module UI = FStar.UInt
+module S = FStar.Seq
 
 #set-options "--fuel 0 --ifuel 0"
 
-private val aux (t:inttype{unsigned t}) (l:secrecy_level) : (xN:sig (bits t){xN.t == int_t t l})
-let aux t l =
-{ t = int_t t l
-; v = (fun x i -> FStar.UInt.nth #(bits t) (v x) i)
-; mk = (fun f -> mk_int (UInt.from_vec #(bits t) (FStar.Seq.init (bits t) f)))
+private val aux (t:inttype{unsigned t}) (l:secrecy_level) (n:nat{n<=bits t}) : foo bool
+let aux t l n =
+{ n = n
+; t = int_t t l
+; v = (fun x i -> UI.nth #(bits t) (v x) i)
+; mk = (fun f -> mk_int (UI.from_vec #(bits t) (S.init (bits t) (fun i -> if i<n then f i else false))))
 ; mk_def = (fun f i -> ())
-; ones_ = Lib.IntTypes.ones t l
-; zeros_ = Lib.IntTypes.zeros t l
-; and_ = logand
-; xor_ = logxor
-; or_ = logor
-; not_ = lognot
-; zeros_spec = (fun i -> UInt.zero_nth_lemma #(bits t) i)
-; ones_spec = (fun i -> UInt.ones_nth_lemma #(bits t) i)
-; and_spec = (fun x y i -> logand_spec x y)
-; xor_spec = (fun x y i -> logxor_spec x y)
-; or_spec = (fun x y i -> logor_spec x y)
-; not_spec = (fun x i -> lognot_spec x)
 }
 
-val bitmap (t:inttype{unsigned t}) (l:secrecy_level) (n:nat) : Type0
-let rec bitmap t l n = if n <= bits t then int_t t l else int_t t l * bitmap t l (n-bits t)
-
-val uN (t:inttype{unsigned t}) (l:secrecy_level) (n:nat{n<=bits t}): (xN:sig n{xN.t == bitmap t l n})
-#push-options "--fuel 1"
+val uN (t:inttype{unsigned t}) (l:secrecy_level) (n:nat{n<=bits t}) : bar
 let uN t l n =
-  if n = bits t then
-    aux t l
-  else
-    xN_rest (aux t l) n
-#pop-options
+{ xN = aux t l n
+; ones_ = ones t l
+; zeros_ = zeros t l
+; and_ = (fun x y -> logand #t #l x y)
+; xor_ = (fun x y -> logxor #t #l x y)
+; or_ = (fun x y -> logor #t #l x y)
+; not_ = (fun x -> lognot #t #l x)
+; ones_spec = (fun i -> UI.ones_nth_lemma #(bits t) i)
+; zeros_spec = (fun i -> UI.zero_nth_lemma #(bits t) i)
+; and_spec = (fun x y i -> logand_spec #t #l x y)
+; xor_spec = (fun x y i -> logxor_spec #t #l x y)
+; or_spec = (fun x y i -> logor_spec #t #l x y)
+; not_spec = (fun x i -> lognot_spec #t #l x)
+}
 
+let uN_zeros_spec (#t:inttype{unsigned t}) (#l:secrecy_level) (#n:nat{n<=bits t}) (i:nat{i<n}) :
+  Lemma ((_).v (uN t l n).zeros_ i == false)
+  = ()
+let uN_ones_spec (#t:inttype{unsigned t}) (#l:secrecy_level) (#n:nat{n<=bits t}) (i:nat{i<n}) :
+  Lemma ((_).v (uN t l n).ones_ i == true)
+  = UI.ones_nth_lemma #(bits t) i
+
+let uN_and_spec #t #l #n (x y:(aux t l n).t) (i:nat{i<n}) :
+  Lemma ((_).v ((uN t l n).and_ x y) i == ((_).v x i && (_).v y i))
+  = logand_spec #t #l x y
+let uN_or_spec #t #l #n (x y:(aux t l n).t) (i:nat{i<n}) :
+  Lemma ((_).v ((uN t l n).or_ x y) i == ((_).v x i || (_).v y i))
+  = logor_spec #t #l x y
+let uN_xor_spec #t #l #n (x y:(aux t l n).t) (i:nat{i<n}) :
+  Lemma ((_).v ((uN t l n).xor_ x y) i == ((_).v x i <> (_).v y i))
+  = logxor_spec #t #l x y
+let uN_not_spec #t #l #n (x:(aux t l n).t) (i:nat{i<n}) :
+  Lemma ((_).v ((uN t l n).not_ x) i == not((_).v x i))
+  = lognot_spec #t #l x
+
+(*
 val uN_eq
   (#t1 #t2:(t:inttype{unsigned t})) (#l:secrecy_level)
   (#n:nat{n<=bits t1 /\ n<=bits t2})
   (x:(uN t1 l n).t) (y:(uN t2 l n).t) : Type0
 let uN_eq x y = forall i. (_).v x i == (_).v y i
 
-val lemma0 (n:nat) (m:nat{n<=m}) (a:FStar.UInt.uint_t n) (i:nat{i<n}) :
-  Lemma (FStar.UInt.size a m /\ FStar.UInt.nth #m a i == FStar.UInt.nth #n a i)
+val lemma0 (n:nat) (m:nat{n<=m}) (a:UI.uint_t n) (i:nat{i<n}) :
+  Lemma (UI.size a m /\ UI.nth #m a i == UI.nth #n a i)
 let rec lemma0 n m a i =
   if n=0 then (
     ()
@@ -58,10 +76,11 @@ let uN_cast #t1 t2 #l #n x =
   let n1 = bits t1 in
   let n2 = bits t2 in
   let a : int_t t1 l = x in
+  assume (PUB? l \/ SEC? l);
   let b : int_t t2 l = cast t2 l a in
   let y : (uN t2 l n).t = b in
-  assert(forall (i:nat{i<n}). (_).v y i == FStar.UInt.nth #n2 (v a % pow2 n2) i);
-  let aux (i:nat{i<n}) : Lemma (FStar.UInt.nth #n2 (v a % pow2 n2) i == FStar.UInt.nth #n1 (v a) i) =
+  assert(forall (i:nat{i<n}). (_).v y i == UI.nth #n2 (v a % pow2 n2) i);
+  let aux (i:nat{i<n}) : Lemma (UI.nth #n2 (v a % pow2 n2) i == UI.nth #n1 (v a) i) =
     if n = 0 then ( ()
     ) else if n2<n1 then (
       lemma0 n2 n1 (v a % pow2 n2) i;
@@ -71,7 +90,7 @@ let uN_cast #t1 t2 #l #n x =
     )
   in
   FStar.Classical.forall_intro aux;
-  assert(forall (i:nat{i<n}). FStar.UInt.nth #n2 (v a % pow2 n2) i == FStar.UInt.nth #n1 (v a) i);
+  assert(forall (i:nat{i<n}). UI.nth #n2 (v a % pow2 n2) i == UI.nth #n1 (v a) i);
   y
 
 val uN_expend (#t:(t:inttype{unsigned t})) (#l:secrecy_level) (#n:nat{n<=bits t}) (m:nat{n<=m /\ m<=bits t}) (x:(uN t l n).t) :
@@ -94,7 +113,7 @@ let uN_shift_left #t #l #n x k =
     if n=0 then
       ()
     else
-      FStar.UInt.shift_left_lemma_2 #(bits t) (v #t #l x) k i
+      UI.shift_left_lemma_2 #(bits t) (v #t #l x) k i
   in
   FStar.Classical.forall_intro aux;
   y
@@ -111,9 +130,9 @@ let uN_shift_right #t #l #n x k =
     if n=0 then (
       ()
     ) else if i<k then (
-      FStar.UInt.shift_right_lemma_1 #(bits t) (v #t #l x) k i
+      UI.shift_right_lemma_1 #(bits t) (v #t #l x) k i
     ) else (
-      FStar.UInt.shift_right_lemma_2 #(bits t) (v #t #l x) k i
+      UI.shift_right_lemma_2 #(bits t) (v #t #l x) k i
     )
   in
   FStar.Classical.forall_intro aux;
@@ -129,17 +148,18 @@ val uN_concat
     (ensures fun z -> forall (i:nat{i<n+n}). (_).v z i == (if i<n then (_).v x i else (_).v y (i-n)))
 #push-options "--z3rlimit 100"
 let uN_concat #t1 #l t2 #n x y =
-  let mask : (uN t2 l (n+n)).t = (_).not_ (uN_shift_right (_).ones_ n) in
-  assert(forall (i:nat{i<n+n}). (_).v mask i == (if i<n then true else false));
+  let mask : (uN t2 l (n+n)).t = uN_not (uN_shift_right uN_ones n) in
+  //assert(forall (i:nat{i<n+n}). (_).v mask i == (if i<n then true else false));
   let x' : (uN t2 l (n+n)).t = uN_expend (n+n) (uN_cast t2 x) in
-  assert (forall (i:nat{i<n+n}). (_).v x' i == (if i<n then (_).v x i else (_).v x' i));
-  let x' : (uN t2 l (n+n)).t = (_).and_ x' mask in
-  assert(forall (i:nat{i<n+n}). (_).v x' i == (if i<n then (_).v x i else false));
+  //assert (forall (i:nat{i<n+n}). (_).v x' i == (if i<n then (_).v x i else (_).v x' i));
+  let x' : (uN t2 l (n+n)).t = uN_and x' mask in
+  //assert(forall (i:nat{i<n+n}). (_).v x' i == (if i<n then (_).v x i else false));
   let y' : (uN t2 l (n+n)).t = uN_expend (n+n) (uN_cast t2 y) in
-  assert(forall (i:nat{i<n+n}). (_).v y' i == (if i<n then (_).v y i else (_).v y' i));
+  //assert(forall (i:nat{i<n+n}). (_).v y' i == (if i<n then (_).v y i else (_).v y' i));
   let y' : (uN t2 l (n+n)).t = uN_shift_right #t2 #l #(n+n) y' n in
-  assert(forall (i:nat{i<n+n}). (_).v y' i == (if i<n then false else (_).v y (i-n)));
-  (_).or_ x' y'
+  //assert(forall (i:nat{i<n+n}). (_).v y' i == (if i<n then false else (_).v y (i-n)));
+  admit ();
+  uN_or x' y'
 #pop-options
 
 val uN_split
@@ -247,15 +267,15 @@ let uNxM_v_split #t #l #n #m x =
   (y, z)
 #pop-options
 
-let foo (n:nat) = (t:inttype{unsigned t /\ n<=bits t})
+let tt (n:nat) = (t:inttype{unsigned t /\ n<=bits t})
 
-type transposable : (n:nat -> foo n -> m:nat -> foo m -> Type0) =
-| Tr1 : t1:foo 1 -> t2:foo 1 -> transposable 1 t1 1 t2
-| TrH : n:nat -> m:nat -> #t1:foo n -> #t2:foo m -> t3:foo (n+n) -> transposable n t1 m t2 -> transposable (n+n) t3 m t2
-| TrV : n:nat -> m:nat -> #t1:foo n -> #t2:foo m -> t3:foo (m+m) -> transposable n t1 m t2 -> transposable n t1 (m+m) t3
+type transposable : (n:nat -> tt n -> m:nat -> tt m -> Type0) =
+| Tr1 : t1:tt 1 -> t2:tt 1 -> transposable 1 t1 1 t2
+| TrH : n:nat -> m:nat -> #t1:tt n -> #t2:tt m -> t3:tt (n+n) -> transposable n t1 m t2 -> transposable (n+n) t3 m t2
+| TrV : n:nat -> m:nat -> #t1:tt n -> #t2:tt m -> t3:tt (m+m) -> transposable n t1 m t2 -> transposable n t1 (m+m) t3
 
 val transpose
-  (#n #m:nat) (#t1:foo n) (#l:secrecy_level) (#t2:foo m)
+  (#n #m:nat) (#t1:tt n) (#l:secrecy_level) (#t2:tt m)
   (pr:transposable n t1 m t2)
   (x:uNxM t1 l n m) :
   Pure (uNxM t2 l m n)
@@ -264,23 +284,24 @@ val transpose
     (decreases pr)
 #push-options "--ifuel 1 --z3rlimit 100"
 let rec transpose #n #m #t1 #l #t2 pr x =
-  match pr with
-  | Tr1 _ _ -> xNxM_mk _ _ (fun 0 -> uN_cast t2 (index x 0))
-  | TrH n m #t3 #t2 t1 pr' ->
-    let (y, z) : (uNxM t3 l n m * uNxM t3 l n m) = uNxM_h_split t3 (x <: uNxM t1 l (n+n) m) in
-    let y' : uNxM t2 l m n = transpose pr' y in
-    let z' : uNxM t2 l m n = transpose pr' z in
-    let w : uNxM t2 l m (n+n) = uNxM_v_concat y' z' in
-    w
-  | TrV n m #t1 #t3 t2 pr' ->
-    let (y, z) : (uNxM t1 l n m * uNxM t1 l n m) = uNxM_v_split (x <: uNxM t1 l n (m+m)) in
-    let y' : uNxM t3 l m n = transpose pr' y in
-    let z' : uNxM t3 l m n = transpose pr' z in
-    let w : uNxM t2 l (m+m) n = uNxM_h_concat t2 y' z' in
-    w
+  admit ()
+  //match pr with
+  //| Tr1 _ _ -> xNxM_mk _ _ (fun 0 -> uN_cast t2 (index x 0))
+  //| TrH n m #t3 #t2 t1 pr' ->
+  //  let (y, z) : (uNxM t3 l n m * uNxM t3 l n m) = uNxM_h_split t3 (x <: uNxM t1 l (n+n) m) in
+  //  let y' : uNxM t2 l m n = transpose pr' y in
+  //  let z' : uNxM t2 l m n = transpose pr' z in
+  //  let w : uNxM t2 l m (n+n) = uNxM_v_concat y' z' in
+  //  w
+  //| TrV n m #t1 #t3 t2 pr' ->
+  //  let (y, z) : (uNxM t1 l n m * uNxM t1 l n m) = uNxM_v_split (x <: uNxM t1 l n (m+m)) in
+  //  let y' : uNxM t3 l m n = transpose pr' y in
+  //  let z' : uNxM t3 l m n = transpose pr' z in
+  //  let w : uNxM t2 l (m+m) n = uNxM_h_concat t2 y' z' in
+  //  w
 #pop-options
 
-val transpose_inv (#n #m:nat) (#t1:foo n) (#t2:foo m) (pr:transposable n t1 m t2) :
+val transpose_inv (#n #m:nat) (#t1:tt n) (#t2:tt m) (pr:transposable n t1 m t2) :
   Pure (transposable m t2 n t1) (requires True) (ensures fun _ -> True) (decreases pr)
 #push-options "--ifuel 1"
 let rec transpose_inv pr = match pr with
@@ -312,13 +333,19 @@ let transpose_8_64 = TrV 8 32 U64 transpose_8_32
 val transpose_64_8 : transposable 64 U64 8 U8
 let transpose_64_8 = transpose_inv transpose_8_64
 
-val line_transpose (#n #m:nat) (#t1:foo n) (#t2:foo m) (#l:secrecy_level) (x:uNxM t1 l n m) (i:nat{i<n})
+val line (#a:Type0) (#xN:foo a) (#m:nat) (i:nat{i<m}) (x:xNxM xN m) : x1xM a xN.n
+let line i x =
+  let aux1 j k = (_).v (index x i) j in
+  let aux2 j = (_).mk (aux1 j) in
+  xNxM_mk _ _ aux2
+
+val line_transpose (#n #m:nat) (#t1:tt n) (#t2:tt m) (#l:secrecy_level) (x:uNxM t1 l n m) (i:nat{i<n})
   (pr:transposable n t1 m t2) :
     Lemma (line i (transpose pr x) == column i x)
   [SMTPat (line i (transpose pr x))]
 let line_transpose x i pr = xNxM_eq_intro (line i (transpose pr x)) (column i x)
 
-val column_transpose (#n #m:nat) (#t1:foo n) (#t2:foo m) (#l:secrecy_level) (x:uNxM t1 l n m) (j:nat{j<m})
+val column_transpose (#n #m:nat) (#t1:tt n) (#t2:tt m) (#l:secrecy_level) (x:uNxM t1 l n m) (j:nat{j<m})
   (pr:transposable n t1 m t2) :
     Lemma (column j (transpose pr x) == line j x)
   [SMTPat (column j (transpose pr x))]
@@ -326,8 +353,9 @@ let column_transpose x j pr = xNxM_eq_intro (column j (transpose pr x)) (line j 
 
 val transpose_transpose
   (#n #m:nat)
-  (#t1:foo n) (#t2:foo m) (#t3:foo n) (#l:secrecy_level)
+  (#t1:tt n) (#t2:tt m) (#t3:tt n) (#l:secrecy_level)
   (x:uNxM t1 l n m) (j:nat{j<m})
   (pr1:transposable n t1 m t2) (pr2:transposable m t2 n t3) :
     Lemma (line j (transpose pr2 (transpose pr1 x)) == line j x)
 let transpose_transpose x j pr1 pr2 = ()
+*)
